examples/malloc.v
@@ -12,7 +12,7 @@ Proof.
     + eapply RuleCmd. eapply RuleAlloc.
     + eapply RuleCmd. eapply RuleAssign.
   - eapply RuleSplit; eauto using rules, rules_atom.
-    eapply RuleConsequence. 2: { eapply RuleCmd. eapply RuleWriteErr. }
+    eapply RuleConsequence. 2: { eapply RuleCmd. eapply RuleStoreErr. }
     + apply null_implies_unmapped.
     + intros ????. solve_eq_set.
 Qed.
